msort_sub.v
@@ -1,0 +1,143 @@
+(******************************************************************)
+(* Mergesort (subset types) *)
+
+From sortalgs Require Import sorted.
+
+Open Scope list_scope.
+Import List.ListNotations.
+
+Require Import Lia.
+Require Import Program.
+
+Lemma lem_sorted_concat_1 {A} {dto : DecTotalOrder A} :
+  forall (l l1 l2 : list A) x y,
+    Permutation l (l1 ++ y :: l2) -> Sorted (x :: l1) -> leb x y ->
+    Sorted (y :: l2) -> Sorted l -> Sorted (x :: l).
+Proof.
+  intros.
+  rewrite lem_lelst_sorted in *.
+  sauto db: lelst inv: -.
+Qed.
+
+Lemma lem_sorted_concat_2 {A} {dto : DecTotalOrder A} :
+  forall (l l1 l2 : list A) x y,
+    Permutation l (x :: l1 ++ l2) -> Sorted (x :: l1) -> leb y x ->
+    Sorted (y :: l2) -> Sorted l -> Sorted (y :: l).
+Proof.
+  intros.
+  rewrite lem_lelst_sorted in *.
+  sauto db: lelst inv: -.
+Qed.
+
+Program Fixpoint merge {A} {dto : DecTotalOrder A}
+  (l1 l2 : {l | Sorted l}) {measure (List.length l1 + List.length l2)} :
+  {l | Sorted l /\ Permutation l (l1 ++ l2)} :=
+  match l1 with
+  | [] => l2
+  | h1 :: t1 =>
+    match l2 with
+    | [] => l1
+    | h2 :: t2 =>
+      if leb_total_dec h1 h2 then
+        h1 :: merge t1 l2
+      else
+        h2 :: merge l1 t2
+    end
+  end.
+Next Obligation.
+  sauto db: list.
+Qed.
+Next Obligation.
+  eauto using lem_sorted_tail.
+Qed.
+Next Obligation.
+  sauto use: lem_sorted_concat_1.
+Qed.
+Next Obligation.
+  eauto using lem_sorted_tail.
+Qed.
+Next Obligation.
+  simpl; lia.
+Qed.
+Next Obligation.
+  split.
+  - sauto use: lem_sorted_concat_2.
+  - simpl_sigma.
+    rewrite List.app_comm_cons.
+    apply Permutation_cons_app.
+    intuition.
+Qed.
+
+Program Fixpoint split {A} (l : list A) {measure (length l)} :
+  { (l1, l2) : list A * list A |
+    length l1 + length l2 = length l /\
+    length l1 <= length l2 + 1 /\ length l2 <= length l1 + 1 /\
+    Permutation l (l1 ++ l2) } :=
+  match l with
+  | [] => ([], [])
+  | [x] => ([x], [])
+  | x :: y :: t =>
+    match split t with
+    | (l1, l2) => (x :: l1, y :: l2)
+    end
+  end.
+Solve Obligations with sauto use: Permutation_cons_app.
+
+Lemma lem_split {A} : forall l : list A,
+    2 <= List.length l ->
+    forall l1 l2, (l1, l2) = ` (split l) ->
+    List.length l1 < List.length l /\
+    List.length l2 < List.length l.
+Proof.
+  sauto.
+Qed.
+
+Ltac use_lem_split :=
+  match goal with
+  | [ H1: [] <> ?l, H2: forall x, [x] <> ?l |- _ ] =>
+    assert (2 <= length l) by
+        (clear - H1 H2; destruct l; hauto depth: 1 inv: list)
+  end;
+  sauto use: @lem_split.
+
+Obligation Tactic := idtac.
+
+Program Fixpoint mergesort {A} {dto : DecTotalOrder A} (l : list A)
+  {measure (List.length l)} : {l' | Sorted l' /\ Permutation l' l} :=
+  match l with
+  | [] => []
+  | [x] => [x]
+  | _ =>
+    match split l with
+    | (l1, l2) => merge (mergesort l1) (mergesort l2)
+    end
+  end.
+Next Obligation.
+  sauto.
+Qed.
+Next Obligation.
+  sauto.
+Qed.
+Next Obligation.
+  program_simpl; use_lem_split.
+Qed.
+Next Obligation.
+  sauto.
+Qed.
+Next Obligation.
+  program_simpl; use_lem_split.
+Qed.
+Next Obligation.
+  sauto.
+Qed.
+Next Obligation.
+  split.
+  - sauto.
+  - qauto use: Permutation_app, Permutation_sym, perm_trans.
+Qed.
+Next Obligation.
+  sauto.
+Qed.
+Next Obligation.
+  program_simpl.
+Defined.
